Fix some diaframe setup
Thanks to Ike for help with this

src/goose_lang/automation/symb_exec_wp.v
@@ -539,6 +539,24 @@ Section abducts.
     HINT1 Q ✱ [MT' $ flip wp_execute_op R' ∘ K ∘ e_out'] ⊫ [id]; P.
   Proof. intros. eapply execution_abduct_lem => //. tc_solve. Qed.
 
+  Class PerennialSpec (e : expr Λ) (TT1 TT2 : tele) (P : TT1 -t> iProp Σ) (Q : TT1 -t> TT2 -t> iProp Σ) (v : TT1 -t> TT2 -t> val Λ) :=
+    perennial_spec_sound Φ : (∃.. tt1, tele_app P tt1 ∗ (∀.. tt2, tele_app (tele_app Q tt1) tt2 -∗ Φ (tele_app (tele_app v tt1) tt2))) ⊢ WP e {{ Φ }}.
+
+  Global Instance perennial_lang_apply_spec e Φ TT1 TT2 P Q v K e_in :
+    ReshapeExprAnd (expr Λ) e K e_in (PerennialSpec e_in TT1 TT2 P Q v) →
+    LanguageCtx K →
+    HINT1 ε₀ ✱ [ ∃.. tt1 : TT1, tele_app P tt1 ∗
+        (∀.. tt2 : TT2, tele_app (tele_app Q tt1) tt2 -∗
+                        WP (K $ of_val (tele_app (tele_app v tt1) tt2)) {{ Φ }} ) ] ⊫
+      [id]; WP e {{ Φ }}.
+  Proof.
+    case => -> He_in HK.
+    unfold Abduct. simpl.
+    iIntros "[_ [%tt1 [HP HQ]]]".
+    iApply wp_bind. iApply He_in.
+    iExists tt1. iFrame.
+  Qed.
+
   Global Instance collect_modal_wp_value s e v Φ E :
     IntoVal e v →
     HINT1 ε₀ ✱ [fupd E E $ Φ v] ⊫ [id]; WP e @ s ; E {{ Φ }} | 10.
